# Factoring

## Difference Of Two Squares

> Watch [a video](https://www.youtube.com/watch?v=_qyVzH3e1dY)

$$
a^2 - b^2 = (a - b)(a + b)
$$

## Difference Of Two Cubes

> Watch [a video](https://www.youtube.com/watch?v=eXjxF1I9o4E)

$$
a^3 - b^3 = (a - b)(a^2 + ab + b^2)
$$

## Sum Of Two Cubes

> See the video above

$$
a^3 + b^3 = (a + b)(a^2 - ab + b^2)
$$

## Factoring With The Quadratic Formula

The best way to show this method is with an example:

**Factor**: $3x^2 - 17x + 20$

First, solve for this expression equal to $0$

$$
3x^2 - 17x + 20 = 0
$$

$$
\implies x
= \frac{17 \pm \sqrt{(-17)^2 - 4(3)(20)}}{2(3)}
= \frac{17 \pm 7}{6}
$$

$$
\implies x = 4 \text{ or } x = \frac{5}{3}
$$

From this you can find that if $x = 4$, then $(x - 4)$ is a factor.
If $x = \frac{5}{3} \implies 3x = 5$, then $(3x - 5)$ is a factor.

$$
\therefore 3x^2 - 17x + 20 = (3x - 5)(x - 4)
$$
